Fixes to insert code, first half of self-refinement of insert_child_list

theories/paris/examples/b_tree_adt.v
@@ -24,18 +24,6 @@ Section b_tree_adt.
   Definition init_ranked_tree : val :=
     λ: "v", ref ((#1, InjL "v")).
 
-  (*
-  Definition select_child : val :=
-    rec: "select" "l",
-        match: "l" with
-        | InjL <> => NONE
-        | InjR "a" =>
-            match: Snd ("a") with
-            | InjL <> => Fst "a"
-            | InjR "_" =>
-                let: "b" = flip ()
-   *)
-
   (* Tries to insert a new child into a list of children. The child list may already be full,
      so we return a pair, where the second component is (optionally)  list of the subset of children
      resulting from splitting the list.
@@ -44,13 +32,23 @@ Section b_tree_adt.
      so for simplicity we just put solely the new element in the second list.
    *)
 
+  (*
   Definition insert_child_list : val :=
     λ: "l" "v",
       if: list_length "l" < #(S max_child_num') then
-        (InjR (list_cons "v" "l"), NONE) 
+        (InjR (list_cons (ref "v") "l"), NONE)
       else
-        (InjR ("l"), SOME (InjR (list_cons "v" list_nil))).
-  
+        (InjR ("l"), SOME (InjR (list_cons (ref "v") list_nil))).
+   *)
+
+  Definition insert_child_list' : val :=
+    λ: "p" "l" "v",
+      if: list_length "l" < #(S max_child_num') then
+        "p" <- InjR (list_cons (ref "v") "l") ;;
+        NONE
+      else
+        SOME (InjR (list_cons (ref "v") list_nil)).
+
   Definition insert_tree_aux : val :=
     rec: "insert_tree" "p" "v" :=
         let: "t" := !"p" in
@@ -66,9 +64,7 @@ Section b_tree_adt.
             | SOME "new" =>
                 (* Either the child was a leaf, or we had to split the child, so
                    we must insert "new" into the current node *)
-                let, ("t'", "opt") := insert_child_list "l" "v" in
-                "p" <- "t'";;
-                "opt"
+                insert_child_list' "p" "l" "v"
             end
         end.
 
@@ -82,6 +78,203 @@ Section b_tree_adt.
           let: "new_root" := InjR (list_cons (ref !"p") (list_cons (ref "t'") list_nil)) in
           "p" <- "new_root"
       end.
-      
+
+
+
+  Context `{!parisGS Σ}.
+
+  Definition btree_ptrv p treev depth tree l : iProp Σ :=
+    ⌜ @is_ab_b_tree max_child_num' depth l tree ⌝ ∗
+        p ↦ treev ∗
+        relate_ab_tree_with_v tree treev.
+
+  Definition btree_ptrv' p treev depth tree l : iProp Σ :=
+    ⌜ @is_ab_b_tree max_child_num' depth l tree ⌝ ∗
+        p ↦ₛ treev ∗
+        relate_ab_tree_with_v' tree treev.
+
+  Definition btree_ptr p depth tree l : iProp Σ :=
+    ∃ treev, btree_ptrv p treev depth tree l.
+
+  Definition btree_ptr' p depth tree l : iProp Σ :=
+    ∃ treev, btree_ptrv' p treev depth tree l.
+
+  Lemma wp_init_tree (v : val) :
+    {{{ True }}}
+      init_tree v
+    {{{ (p : loc), RET (#p); btree_ptr p O (Lf v) [Some v] }}}.
+  Proof.
+    iIntros (Φ) "_ HΦ".
+    rewrite /init_tree. wp_pures. wp_alloc p as "Hp".
+    iModIntro. iApply "HΦ". iFrame.
+    iSplit.
+    { iPureIntro. econstructor. }
+    { rewrite relate_ab_tree_with_v_Lf //=. }
+  Qed.
+
+  Lemma spec_init_tree (v: val) K E:
+    ⤇ fill K (init_tree v) -∗ spec_update E (∃ (p:loc), ⤇ fill K #p ∗ btree_ptr' p O (Lf v) [Some v]).
+  Proof.
+    iIntros "H".
+    rewrite /init_tree. tp_pures.
+    tp_alloc as p "Hp".
+    iModIntro. iExists _. iFrame.
+    iSplit.
+    { iPureIntro. econstructor. }
+    { rewrite relate_ab_tree_with_v_Lf' //=. }
+  Qed.
+
+  Lemma rel_insert_child_list' K p p' ltv ltv' depth l vs vs2 t tv tv' :
+    {{{ btree_ptrv p (InjRV ltv) (S depth) (Br l) vs ∗
+        btree_ptrv' p' (InjRV ltv') (S depth) (Br l) vs ∗
+        ⌜ @is_ab_b_tree max_child_num' depth vs2 t ⌝ ∗
+        relate_ab_tree_with_v t tv ∗
+        relate_ab_tree_with_v' t tv' ∗
+        ⤇ fill K (insert_child_list' #p' ltv' tv')
+    }}}
+      insert_child_list' #p ltv tv
+    {{{ res, RET res;
+        ∃ ltv ltv' vs l' (res' : val),
+        ⤇ fill K res' ∗
+          btree_ptrv p ltv (S depth) (Br l') vs ∗
+          btree_ptrv' p' ltv' (S depth) (Br l') vs ∗
+          ((⌜ res = NONEV ⌝ ∗ ⌜ res' = NONEV ⌝) ∨ True)
+    }}}.
+  Proof.
+    iIntros (Φ) "(Hbtree&Hbtree'&%Htwf&Htv&Htv'&Hspec) HΦ".
+    rewrite /insert_child_list'.
+    wp_pures.
+    tp_pures.
+    iDestruct "Hbtree" as "(%Hwft0&Hp&Hrelate)".
+    iDestruct "Hbtree'" as "(%Hwft0'&Hp'&Hrelate')".
+    iEval (rewrite relate_ab_tree_with_v_Br) in "Hrelate".
+    iEval (rewrite relate_ab_tree_with_v_Br') in "Hrelate'".
+    iDestruct "Hrelate" as (??? Heq1 Heq2 Heq3 ?) "(H1&H2)".
+    inversion Heq1; subst.
+    iDestruct "Hrelate'" as (??? Heq1' Heq2' Heq3' ?) "(H1'&H2')".
+    inversion Heq1'; subst.
+    wp_apply (wp_list_length); eauto.
+    iIntros (? ->).
+    tp_bind (list_length _)%E.
+    iMod (spec_list_length with "[//] Hspec") as (?) "(Hspec&->)". simpl.
+    wp_pures.
+    case_bool_decide.
+    - tp_pures. rewrite bool_decide_true; last by lia.
+      wp_pures. tp_pures.
+      wp_alloc ptrv as "Hptv".
+      replace (#ptrv) with (inject ptrv) by auto.
+      wp_apply (wp_list_cons); eauto.
+      iIntros (? Hlist).
+      tp_alloc as ptrv' "Hptv'".
+      tp_bind (list_cons _ _)%E.
+      replace (#ptrv') with (inject ptrv') by auto.
+      iMod (spec_list_cons with "[] Hspec") as (?) "(Hspec&%Hlist')".
+      { eauto. }
+      simpl.
+      tp_pures. tp_store. tp_pures.
+      wp_store. wp_pures.
+      iApply "HΦ".
+      iModIntro.
+      inversion Hwft0.
+      (* FIX vs' --> it should be the things from is_ab_b_tree of t, -1 of the replicated sets of 0s *)
+      set (l0' := ((vs2, t) :: l0)).
+      set (vs' :=
+              flat_map (λ x : list (option val), x) l0'.*1 ++
+       replicate ((S max_child_num' - length l0') * S max_child_num' ^ depth) None).
+      set (l' := (snd <$> l0')).
+      iExists _, _, vs', l', _.
+      iFrame "Hspec".
+      rewrite /btree_ptrv/btree_ptrv'.
+      iFrame "Hp Hp'".
+      iSplitL "Hptv Htv H1 H2".
+      { iSplit.
+        * iPureIntro. rewrite /l'/vs'. econstructor.
+          ** rewrite /l0'. econstructor; eauto.
+          ** rewrite /l0'. simpl. split; first lia.
+             rewrite /b_tree.max_child_num.
+             cut (length l0 = length l); first by lia.
+             subst. rewrite map_length //.
+        * rewrite relate_ab_tree_with_v_Br. iExists _, (ptrv :: loc_lis), (tv :: v_lis).
+          iSplit; first eauto.
+          iSplit.
+          { iPureIntro; rewrite /l'/l0'. rewrite fmap_cons ?cons_length. congruence. }
+          iSplit.
+          { iPureIntro; rewrite /l'/l0'. rewrite fmap_cons ?cons_length. congruence. }
+          iSplit; first done.
+          simpl. iFrame.
+      }
+      iSplitL "Hptv' Htv' H1' H2'".
+      { iSplit.
+        * iPureIntro. rewrite /l'/vs'. econstructor.
+          ** rewrite /l0'. econstructor; eauto.
+          ** rewrite /l0'. simpl. split; first lia.
+             rewrite /b_tree.max_child_num.
+             cut (length l0 = length l); first by lia.
+             subst. rewrite map_length //.
+        * rewrite relate_ab_tree_with_v_Br'. iExists _, (ptrv' :: loc_lis0), (tv' :: v_lis0).
+          iSplit; first eauto.
+          iSplit.
+          { iPureIntro; rewrite /l'/l0'. rewrite fmap_cons ?cons_length. congruence. }
+          iSplit.
+          { iPureIntro; rewrite /l'/l0'. rewrite fmap_cons ?cons_length. congruence. }
+          iSplit; first done.
+          simpl. iFrame.
+      }
+      eauto.
+    -
+  Abort.
+
+   (* Specifying the unary behavior would be handy, since then we
+   could cut out on having to effectively do the proof as many
+   redundant times, but it's annoying to do so because we would have
+   to specify its behavior quite specifically. *)
+
+  (*
+  Lemma wp_insert_child_list' p lsv v depth vs1 vs2 ls t:
+    {{{ btree_ptrv p (InjRV lsv) (S depth) (Br ls) vs2 ∗
+        ⌜ @is_ab_b_tree max_child_num' depth vs1 t ⌝ ∗
+        relate_ab_tree_with_v t v
+    }}}
+      insert_child_list' #p lsv v
+    {{{ res, RET res;
+        if decide (length ls < S max_child_num')%nat then
+          ⌜ res = NONEV ⌝ ∗ btree_ptrv p (InjRV (v, lsv)) depth (Br (t :: ls)) (vs1 ++ vs2)
+        else
+          True }}}.
+  Proof.
+    iIntros (Φ) "(Hbtree_ptrv&%Htwf&Htv) HΦ".
+    rewrite /insert_child_list'.
+    wp_pures.
+    iDestruct "Hbtree_ptrv" as "(%Hwft'&Hp&Hrelate)".
+    iEval (rewrite relate_ab_tree_with_v_Br) in "Hrelate".
+    iDestruct "Hrelate" as (??? Heq1 Heq2 Heq3 ?) "(H1&H2)".
+    inversion Heq1; subst.
+    wp_apply (wp_list_length); eauto.
+    iIntros (? ->).
+    wp_pures. case_bool_decide.
+    { wp_pures.
+      wp_alloc lv as "Hlv".
+      replace (#lv) with (inject lv) by auto.
+      wp_apply (wp_list_cons); eauto.
+      iIntros (? Hlist).
+      wp_store.
+      wp_pures.
+      iModIntro. iApply "HΦ".
+      rewrite decide_True; last first.
+      { lia. }
+      iSplit; auto.
+      rewrite /btree_ptrv.
+      iSplit.
+      { iPureIntro.
+        inversion Hwft'.
+        Print is_ab_b_tree.
+        simpl.
+        eapply (is_ab_b_tree_br _ ((vs1, t) :: _)).
+        econstructor. simpl.
+      simpl.
+      iFrame.
+      iExists _.
+      wp_pures.
+   *)
 
 End b_tree_adt.
